theories/CounterMachines/CM2X.v
@@ -1,0 +1,58 @@
+(* 
+  Problem(s):
+    Two Counter Machine with Swap Halting (CM2X_HALT)
+
+  Literature:
+    [1, Problem 14.2-2] Minsky, Marvin Lee. Computation. Englewood Cliffs: Prentice-Hall, 1967.
+*)
+
+Require Import List ssrfun.
+
+(* a configuration consists of a program index and two counter values *)
+Notation Config := (nat * (nat * nat))%type.
+
+(* the instruction inc maps 
+      a configuration (i, (a, b)) to (1+i, (b, 1+a))
+    an instruction dec j maps
+      a configuration (i, (0, b)) to (1+i, (b, 0)) 
+      a configuration (i, (1+a, b)) to (j, (b, a))  *)
+Inductive Instruction : Set := 
+  | inc : Instruction
+  | dec : nat -> Instruction.
+
+(* a two counter machine with swap is a list of instructions *)
+Notation Cm2x := (list Instruction).
+
+(* two counter machine with swap step function *)
+Definition step (M: Cm2x) (x: Config) : option Config :=
+  let '(i, (a, b)) := x in
+  match nth_error M i with
+  | None => None (* halting configuration *)
+  | Some inc => Some (1+i, (b, 1+a))
+  | Some (dec j) => Some (
+    match a with
+    | 0 => (1+i, (b, 0))
+    | S n => (j, (b, n))
+    end)
+  end.
+
+(* unfold step if the configuration is decomposed *)
+Arguments step _ !x /.
+
+(* iterated partial two-counter machine step function *)
+Definition steps (M: Cm2x) (k: nat) (x: Config) : option Config :=
+  Nat.iter k (obind (step M)) (Some x).
+
+(* configuration reachability *)
+Definition reaches (M: Cm2x) (x y: Config) :=
+  exists k, steps M k x = Some y.
+
+(* does M eventually terminate starting from the configuration x? *)
+Definition terminating (M: Cm2x) (x: Config) :=
+  exists k, steps M k x = None.
+
+(* Two-counter Machine with Swap Halting:
+   Given a two-counter machine with swap M,
+   does a run in M starting from configuration (0, (0, 0)) eventually halt? *)
+Definition CM2X_HALT : Cm2x -> Prop :=
+  fun M => terminating M (0, (0, 0)).
