theories/IntersectionTypes/CD.v
@@ -22,10 +22,10 @@ Inductive type_assignment (Gamma : list ty) : tm -> sty -> Prop :=
       In t (s::phi) ->
       type_assignment Gamma (var x) t
   | type_assignment_app M N s phi t :
-    type_assignment Gamma M (arr s phi t) ->
-    type_assignment Gamma N s ->
-    Forall (type_assignment Gamma N) phi ->
-    type_assignment Gamma (app M N) t
+      type_assignment Gamma M (arr s phi t) ->
+      type_assignment Gamma N s ->
+      Forall (type_assignment Gamma N) phi ->
+      type_assignment Gamma (app M N) t
   | type_assignment_arr M s phi t :
       type_assignment ((s, phi) :: Gamma) M t ->
       type_assignment Gamma (lam M) (arr s phi t).
